dm4good/README.md
@@ -4,8 +4,6 @@ Should work fine with Coq 8.14.
 
 ## TODO
 
-- Refactor to define a notion of monad and `ReqMonad` and `DijkstraMonad` on
-top of it.
 - Show that `pure_wp` also has a lift from pure for ND.
 - Next step is the guarded construction and then use it for stuff like ND and
 maybe IO?
